src/Arithmetic/MontgomeryReduction/WordByWord/Definition.v
@@ -19,32 +19,29 @@ Section WordByWordMontgomery.
   Context
     {r : positive}
     {R_numlimbs : nat}
-    (N' : T R_numlimbs).
-  (** TODO(andreser): Add a comment here about why we take in [N : T
-       R_numlimbs]; we need [N : T (S R_numlimbs)] so that the limb
-       arithmetic works out exactly (so that we can add [q * N] of
-       length [S (S R_numlimbs)] to [S1] of length [S (S R_numlimbs)]
-       and then do [divmod] to get something of length [S
-       R_numlimbs]. *)
-  Local Notation N := (join0 N').
+    (N : T R_numlimbs).
+
+  Local Notation scmul := (@scmul (Z.pos r)).
+  Local Notation add' := (fun n => @add (Z.pos r) (S n) n (S n)).
+  Local Notation add := (fun n => @add (Z.pos r) n n n).
 
   Definition redc_body_no_cps (B : T R_numlimbs) (k : Z) {pred_A_numlimbs} (A_S : T (S pred_A_numlimbs) * T (S R_numlimbs))
     : T pred_A_numlimbs * T (S R_numlimbs)
-    := @redc_body T (@divmod) r R_numlimbs (@scmul (Z.pos r)) (@add (Z.pos r)) (@drop_high (S R_numlimbs)) N B k _ A_S.
+    := @redc_body T (@divmod) r R_numlimbs (@scmul) add add' (@drop_high (S R_numlimbs)) N B k _ A_S.
   Definition redc_loop_no_cps (B : T R_numlimbs) (k : Z) (count : nat) (A_S : T count * T (S R_numlimbs))
     : T 0 * T (S R_numlimbs)
-    := @redc_loop T (@divmod) r R_numlimbs (@scmul (Z.pos r)) (@add (Z.pos r)) (@drop_high (S R_numlimbs)) N B k count A_S.
+    := @redc_loop T (@divmod) r R_numlimbs (@scmul) add add' (@drop_high (S R_numlimbs)) N B k count A_S.
   Definition redc_no_cps {A_numlimbs} (A : T A_numlimbs) (B : T R_numlimbs) (k : Z) : T (S R_numlimbs)
-    := @redc T (@zero) (@divmod) r R_numlimbs (@scmul (Z.pos r)) (@add (Z.pos r)) (@drop_high (S R_numlimbs)) N _ A B k.
+    := @redc T (@zero) (@divmod) r R_numlimbs (@scmul) add add' (@drop_high (S R_numlimbs)) N _ A B k.
 
   Definition redc_body_cps {pred_A_numlimbs} (A : T (S pred_A_numlimbs)) (B : T R_numlimbs) (k : Z) (S' : T (S R_numlimbs))
              {cpsT} (rest : T pred_A_numlimbs * T (S R_numlimbs) -> cpsT)
     : cpsT
     := divmod_cps A (fun '(A, a) =>
-       @scmul_cps r _ a B _ (fun aB => @add_cps r _ S' aB _ (fun S1 =>
+       @scmul_cps r _ a B _ (fun aB => @add_cps r _ _ (S R_numlimbs) S' aB _ (fun S1 =>
        divmod_cps S1 (fun '(_, s) =>
        dlet q := fst (Z.mul_split r s k) in
-       @scmul_cps r _ q N _ (fun qN => @add_cps r _ S1 qN _ (fun S2 =>
+       @scmul_cps r _ q N _ (fun qN => @add_cps r _ _ _ S1 qN _ (fun S2 =>
        divmod_cps S2 (fun '(S3, _) =>
        @drop_high_cps (S R_numlimbs) S3 _ (fun S4 => rest (A, S4))))))))).
 
